Prove that srd implies functional liveness!

IL/LabelsDefined.v
@@ -3,6 +3,7 @@ Require Import Util Relations Get Drop Var Val Exp Env Map CSet AutoIndTac MoreL
 
 Set Implicit Arguments.
 
+
 Inductive labelsDefined : stmt -> nat -> Prop :=
   | labelsDefinedExp x e s L
     : labelsDefined s L
@@ -23,6 +24,7 @@ Inductive labelsDefined : stmt -> nat -> Prop :=
     :  labelsDefined s (S L)
       -> labelsDefined t (S L)
       -> labelsDefined (stmtFun Z s t) L.
+
 
 Inductive paramsMatch : stmt -> list nat -> Prop :=
   | paramsMatchExp x e s L
@@ -45,6 +47,54 @@ Inductive paramsMatch : stmt -> list nat -> Prop :=
     :  paramsMatch s (length Z::L)
       -> paramsMatch t (length Z::L)
       -> paramsMatch (stmtFun Z s t) L.
+
+
+Inductive isCalled : stmt -> lab -> Prop :=
+  | IsCalledExp x e s l
+    : isCalled s l
+      -> isCalled (stmtLet x e s) l
+  | IsCalledIf1 e s t l
+    : isCalled s l
+      -> isCalled (stmtIf e s t) l
+  | IsCalledIf2 e s t l
+    : isCalled t l
+      -> isCalled (stmtIf e s t) l
+  | IsCalledGoto f Y
+    : isCalled (stmtApp f Y) f
+  | IsCalledExtern x f Y s l
+    : isCalled s l
+      -> isCalled (stmtExtern x f Y s) l
+  | IsCalledLet1 s t Z l
+    : isCalled s (incc l 1)
+      -> isCalled t (LabI 0)
+      -> isCalled (stmtFun Z s t) l
+  | IsCalledLet s t Z l
+    : isCalled t (incc l 1)
+      -> isCalled (stmtFun Z s t) l.
+
+
+Inductive isFreeLab : stmt -> lab -> Prop :=
+  | IsFreeLabExp x e s l
+    : isFreeLab s l
+      -> isFreeLab (stmtLet x e s) l
+  | IsFreeLabIf1 e s t l
+    : isFreeLab s l
+      -> isFreeLab (stmtIf e s t) l
+  | IsFreeLabIf2 e s t l
+    : isFreeLab t l
+      -> isFreeLab (stmtIf e s t) l
+  | IsFreeLabGoto f Y
+    : isFreeLab (stmtApp f Y) f
+  | IsFreeLabExtern x f Y s l
+    : isFreeLab s l
+      -> isFreeLab (stmtExtern x f Y s) l
+  | IsFreeLabLet1 s t Z l
+    : isFreeLab s (incc l 1)
+      -> isFreeLab (stmtFun Z s t) l
+  | IsFreeLabLet s t Z l
+    : isFreeLab t (incc l 1)
+      -> isFreeLab (stmtFun Z s t) l.
+
 
 (*
 *** Local Variables: ***
